LeanColls/Classes/IndexType/Instances.lean
@@ -1,0 +1,9 @@
+import LeanColls.Classes.IndexType.Basic
+
+open LeanColls
+
+deriving instance IndexType for Bool
+deriving instance IndexType for UInt8
+deriving instance IndexType for UInt16
+deriving instance IndexType for UInt32
+deriving instance IndexType for UInt64
